refactor: pull more axioms into the SSA typeclass; introduce SSADenote for denotations

EffectSSA/ProofSketch/Assumptions.lean
@@ -2,10 +2,19 @@ module
 
 public import EffectSSA.ProofSketch.VarSet
 public import EffectSSA.ProofSketch.Denote
+public import EffectSSA.ProofSketch.Notation.Refinement
 
 namespace EffectSSA.ProofSketch
+public section
 
-public class SSA (ι : Type) (σ : outParam Type) : Type where
+class SSA (ι : Type) (σ : outParam Type) (ν : outParam Type) : Type where
   [decidableEq : DecidableEq ι]
   args : ι → VarSet
   results : ι → VarSet
+  initialState : σ
+  [stateRefine : Refinement σ]
+  [valRefine : Refinement ν]
+
+attribute [implicit_reducible, instance] SSA.stateRefine SSA.valRefine SSA.decidableEq
+
+end
