EffectSSA/ProofSketch/LocalStack.lean
@@ -1,8 +1,9 @@
 module
 
 public import EffectSSA.ProofSketch.VarSet
+public import EffectSSA.ProofSketch.Assumptions
 
-import Std.Data.HashMap
+public import Std.Data.HashMap
 
 /-!
 # LocalStack Structure
@@ -15,11 +16,8 @@ public section
 
 open Std (HashMap)
 
-/-- `Val` is the type of runtime values -/
-axiom Val : Type
-
-def LocalStack.Raw :=
-  @Quot (Std.HashMap VarId Val) Std.HashMap.Equiv
+def LocalStack.Raw (ν) :=
+  @Quot (Std.HashMap VarId ν) Std.HashMap.Equiv
 
 
 /-!
@@ -28,49 +26,50 @@ def LocalStack.Raw :=
 -/
 
 open LocalStack (Raw) in
-structure LocalStack where
-  raw : Raw
+structure LocalStack (ν) where
+  raw : Raw ν
 
 namespace LocalStack
+variable {ν}
 
-def empty : LocalStack where
+def empty : LocalStack ν where
   raw := Quot.mk _ (.mk {})
-instance : EmptyCollection LocalStack where emptyCollection := empty
+instance : EmptyCollection (LocalStack ν) where emptyCollection := empty
 
-def contains (s : LocalStack) (v : VarId) : Bool :=
+def contains (s : LocalStack ν) (v : VarId) : Bool :=
   Quot.lift (·.contains v) (fun _ _ h => h.contains_eq) s.raw
 
-instance : Membership VarId LocalStack where
+instance : Membership VarId (LocalStack ν) where
   mem s v := s.contains v
-instance (v : VarId) (s : LocalStack) : Decidable (v ∈ s) :=
+instance (v : VarId) (s : LocalStack ν) : Decidable (v ∈ s) :=
   inferInstanceAs <| Decidable (s.contains v)
 
 @[simp, grind =]
-theorem mem_iff (s : LocalStack) (v : VarId) : v ∈ s ↔ s.contains v := by rfl
+theorem mem_iff (s : LocalStack ν) (v : VarId) : v ∈ s ↔ s.contains v := by rfl
 
-def get? (s : LocalStack) (v : VarId) : Option Val :=
-  (Quot.lift (fun m : HashMap VarId Val => m[v]?) · s.raw) <| by
+def get? (s : LocalStack ν) (v : VarId) : Option ν :=
+  (Quot.lift (fun m : HashMap VarId ν => m[v]?) · s.raw) <| by
     intro a b hab; exact hab.getElem?_eq
 
-def get (s : LocalStack) (v : VarId) (h : v ∈ s) : Val :=
+def get (s : LocalStack ν) (v : VarId) (h : v ∈ s) : ν :=
   (s.get? v).get <| by
     obtain ⟨raw⟩ := s
     cases raw using Quot.ind
     case mk m =>
       exact HashMap.mem_iff_isSome_getElem?.mp h
 
-instance : GetElem?  LocalStack VarId Val (fun s v => v ∈ s) where
+instance : GetElem? (LocalStack ν) VarId ν (fun s v => v ∈ s) where
   getElem := get
   getElem? := get?
 
-def insert (s : LocalStack) (v : VarId) (x : Val) : LocalStack where
+def insert (s : LocalStack ν) (v : VarId) (x : ν) : LocalStack ν where
   raw := Quot.lift (fun m => Quot.mk _ (m.insert v x))
     (fun _ _ h => Quot.sound (h.insert v x)) s.raw
 
 section Lemmas
 
 @[ext, grind ext]
-theorem ext {s t : LocalStack} : (h : ∀ v : VarId, s[v]? = t[v]?) → s = t := by
+theorem ext {s t : LocalStack ν} : (h : ∀ v : VarId, s[v]? = t[v]?) → s = t := by
   rcases s with ⟨s⟩
   cases s using Quot.ind
   case mk s =>
@@ -91,16 +90,17 @@ end LocalStack
 -/
 @[expose] public section Expose
 
-abbrev LocalStackT := StateT LocalStack
+
+abbrev LocalStackT ν := StateT (LocalStack ν)
 
 namespace LocalStackT
-variable {m} [Monad m]
+variable {m} [Monad m] {ν}
 
 /--
 Read the value of variable `v` from the monadic state,
 returning `none` if `v` has no value assigned.
 -/
-def read? (v : VarId) : LocalStackT m (Option Val) := do
+def read? (v : VarId) : LocalStackT ν m (Option ν) := do
   let ρ ← get
   return ρ[v]?
 
@@ -109,7 +109,7 @@ Assign value `x` to variable `v` in the monadic state.
 
 This is infallible, overwriting any value already present.
 -/
-def push (var : VarId) (val : Val) : LocalStackT m Unit :=
+def push (var : VarId) (val : ν) : LocalStackT ν m Unit :=
   modify (·.insert var val)
   -- NOTE: it seems tempting to throw an error here if `x` is already defined.
   -- However, since we never remove variables, a variable being defined twice
